Redesign k8s RA

src/proof/algebra/kview.v
@@ -4,15 +4,28 @@ From New.proof.k8s_io.apimachinery.pkg.apis.meta Require Export v1_init.
 From iris.algebra Require Import cmra gset gmap.
 From iris.base_logic.lib Require Import own.
 
+(* Reserved names are classified statically. In particular, API-server
+   generated names never satisfy this predicate. *)
+Axiom reserved_key_pred : KKey.t → Prop.
+
+Inductive reservation_status :=
+  | Available
+  | Unavailable.
+
+#[global] Instance reservation_status_eq_decision : EqDecision reservation_status.
+Proof. solve_decision. Defined.
 
 Section kview.
 
-Definition authO : ofe := prodO (gmapO KKey.t (leibnizO KObjectV.t)) (gsetO (leibnizO types.UID.t)).
+Definition authO : ofe :=
+  prodO (gmapO KKey.t (leibnizO KObjectV.t))
+    (gsetO (leibnizO types.UID.t)).
 
 Definition metaUR : ucmra := gmapUR (KKey.t * types.UID.t) (prodR dfracR (agreeR (leibnizO ObjectMetaV.t))).
 Definition specUR : ucmra := gmapUR (KKey.t * types.UID.t) (prodR dfracR (agreeR (leibnizO ObjectSpecV.t))).
 Definition statusUR : ucmra := gmapUR (KKey.t * types.UID.t) (prodR dfracR (agreeR (leibnizO ObjectStatusV.t))).
-Definition fragUR : ucmra := prodUR metaUR (prodUR specUR statusUR).
+Definition reservationUR : ucmra := gmapUR KKey.t (prodR dfracR (agreeR (leibnizO reservation_status))).
+Definition fragUR : ucmra := prodUR metaUR (prodUR specUR (prodUR statusUR reservationUR)).
 
 Implicit Types (a : authO) (b : fragUR).
 
@@ -21,7 +34,8 @@ Local Definition proj_used_uid a : gset types.UID.t := snd a.
 
 Local Definition proj_meta b : metaUR := fst b.
 Local Definition proj_spec b : specUR := fst (snd b).
-Local Definition proj_status b : statusUR := snd (snd b).
+Local Definition proj_status b : statusUR := fst (snd (snd b)).
+Local Definition proj_reservation b : reservationUR := snd (snd (snd b)).
 
 Local Definition valid_kauth a : Prop :=
   map_Forall (λ k obj,
@@ -59,7 +73,17 @@ Local Definition compatible_kfrag b a : Prop :=
       ∀ obj, proj_state a !! k = Some obj →
         (KObjectV.objectmeta obj).(ObjectMetaV.UID') = uid →
         KObjectV.status obj = status
-  ) (proj_status b).
+  ) (proj_status b) ∧
+  map_Forall (λ k '(dq, agree_reservation),
+    ∃ status,
+      agree_reservation ≡ to_agree (A := leibnizO reservation_status) status ∧
+      ✓ dq ∧
+      reserved_key_pred k ∧
+      match status with
+      | Available => proj_state a !! k = None
+      | Unavailable => is_Some (proj_state a !! k)
+      end
+  ) (proj_reservation b).
 
 Local Definition view_rel_raw (n: nat) a b :=
   valid_kauth a ∧ compatible_kfrag b a.
@@ -71,7 +95,7 @@ Local Lemma view_rel_raw_mono n1 n2 a1 a2 b1 b2 :
   (n2 ≤ n1)%nat →
   view_rel_raw n2 a2 b2.
 Proof.
-  intros [Hvalid [Hmeta [Hspec Hstatus]]] Ha Hb _.
+  intros [Hvalid [Hmeta [Hspec [Hstatus Hreservation]]]] Ha Hb _.
   destruct a1 as [state1 used1], a2 as [state2 used2].
   simpl in *.
   destruct Ha as [Hstate Hused].
@@ -94,7 +118,8 @@ Proof.
   assert (Hused_elem : ∀ uid, uid ∈ used1 ↔ uid ∈ used2).
   { exact (proj1 (set_equiv used1 used2) Hused_eqv). }
   apply pair_includedN in Hb as [Hmeta_incl Hrest].
-  apply pair_includedN in Hrest as [Hspec_incl Hstatus_incl].
+  apply pair_includedN in Hrest as [Hspec_incl Hrest].
+  apply pair_includedN in Hrest as [Hstatus_incl Hreservation_incl].
   split.
   { rewrite /valid_kauth.
     rewrite map_Forall_lookup.
@@ -189,7 +214,8 @@ Proof.
       * split.
         { apply (proj1 (Hused_elem _)). exact Huid_in. }
         { split; [exact Hvdq2|exact Hspec_obj]. }
-    + rewrite map_Forall_lookup.
+    + split.
+      * rewrite map_Forall_lookup.
       intros [k uid] [dq2 agree2] Hlookup2.
       destruct (lookup_includedN n2 (proj_status b2) (proj_status b1)) as [Hlookup_incl _].
       specialize (Hlookup_incl Hstatus_incl (k, uid)).
@@ -224,18 +250,61 @@ Proof.
         as Hagree2_n2.
       exists status.
       split.
-      * apply (proj2 (discrete_iff n2 agree2
+      { apply (proj2 (discrete_iff n2 agree2
           (to_agree (A := leibnizO ObjectStatusV.t) status))).
-        etrans; [exact Hagree2_n2|exact (Hagree1 n2)].
-      * split.
+        etrans; [exact Hagree2_n2|exact (Hagree1 n2)]. }
+      { split.
         { apply (proj1 (Hused_elem _)). exact Huid_in. }
-        { split; [exact Hvdq2|exact Hstatus_obj]. }
+        { split; [exact Hvdq2|exact Hstatus_obj]. } }
+      * rewrite map_Forall_lookup.
+        intros k [dq2 agree2] Hlookup2.
+        destruct (lookup_includedN n2 (proj_reservation b2)
+          (proj_reservation b1)) as [Hlookup_incl _].
+        specialize (Hlookup_incl Hreservation_incl k).
+        rewrite Hlookup2 in Hlookup_incl.
+        destruct (Some_includedN_is_Some _ _ _ Hlookup_incl) as
+          [[dq1 agree1] Hlookup1].
+        destruct (Hreservation _ _ Hlookup1) as
+          (status & Hagree1 & Hvdq1 & Hreserved1 & Hstatus_state).
+        rewrite Hlookup1 in Hlookup_incl.
+        assert (Hval1_n2 :
+          ✓{n2} (Some (dq1, agree1) :
+            option (dfrac * agree (leibnizO reservation_status)))).
+        { simpl. apply cmra_valid_validN.
+          apply pair_valid. split; [done|].
+          rewrite Hagree1. done.
+        }
+        assert (Hval2_n2 :
+          ✓{n2} (Some (dq2, agree2) :
+            option (dfrac * agree (leibnizO reservation_status)))).
+        { eapply cmra_validN_includedN; done. }
+        assert (Hvdq2_n2 : ✓{n2} dq2).
+        { apply (proj1 (pair_validN dq2 agree2 n2)).
+          simpl in Hval2_n2. done.
+        }
+        assert (Hvdq2 : ✓ dq2).
+        { by apply (proj2 (cmra_discrete_valid_iff n2 dq2)). }
+        pose proof (Some_pair_includedN _ _ _ _ _ Hlookup_incl) as
+          [_ Hagree_opt_incl].
+        pose proof (proj1 (Some_includedN_total n2 agree2 agree1)
+          Hagree_opt_incl) as Hagree_incl.
+        assert (Hagree1_n2 : ✓{n2} agree1).
+        { rewrite Hagree1. done. }
+        pose proof (agree_valid_includedN n2 agree2 agree1 Hagree1_n2
+          Hagree_incl) as Hagree2_n2.
+        exists status.
+        split.
+        { apply (proj2 (discrete_iff n2 agree2
+            (to_agree (A := leibnizO reservation_status) status))).
+          etrans; [exact Hagree2_n2|exact (Hagree1 n2)].
+        }
+        split_and!; done.
 Qed.
 
 Local Lemma view_rel_raw_valid n a b :
   view_rel_raw n a b → ✓{n} b.
 Proof.
-  intros [_ [Hmeta [Hspec Hstatus]]].
+  intros [_ [Hmeta [Hspec [Hstatus Hreservation]]]].
   apply pair_validN. split.
   - intros [k uid].
     destruct (proj_meta b !! (k, uid)) as [[dq agree_meta]|] eqn:Hlookup.
@@ -258,16 +327,30 @@ Proof.
         { apply cmra_valid_validN. done. }
         { rewrite Hagree. done. }
       * rewrite Hlookup. done.
-    + intros [k uid].
-      destruct (proj_status b !! (k, uid)) as [[dq agree_status]|] eqn:Hlookup.
-      * pose proof (map_Forall_lookup_1 _ _ _ _ Hstatus Hlookup) as Hstatus_i.
+    + apply pair_validN. split.
+      * intros [k uid].
+        destruct (proj_status b !! (k, uid)) as [[dq agree_status]|] eqn:Hlookup.
+        { pose proof (map_Forall_lookup_1 _ _ _ _ Hstatus Hlookup) as Hstatus_i.
         simpl in Hstatus_i.
         destruct Hstatus_i as (status & Hagree & _ & Hvdq & _).
         rewrite Hlookup.
         apply pair_validN. split.
         { apply cmra_valid_validN. done. }
-        { rewrite Hagree. done. }
-      * rewrite Hlookup. done.
+          { rewrite Hagree. done. } }
+        { rewrite Hlookup. done. }
+      * intros k.
+        destruct (proj_reservation b !! k) as [[dq agree_reservation]|]
+          eqn:Hlookup.
+        { pose proof (map_Forall_lookup_1 _ _ _ _ Hreservation Hlookup)
+            as Hreservation_i.
+          simpl in Hreservation_i.
+          destruct Hreservation_i as (status & Hagree & Hvdq & _).
+          rewrite Hlookup.
+          apply pair_validN. split.
+          - apply cmra_valid_validN. done.
+          - rewrite Hagree. done.
+        }
+        { rewrite Hlookup. done. }
 Qed.
 
 Local Lemma view_rel_raw_unit n :
@@ -275,9 +358,10 @@ Local Lemma view_rel_raw_unit n :
 Proof.
   exists ((∅ : gmap KKey.t KObjectV.t), (∅ : gset types.UID.t)).
   split.
-  1: rewrite /valid_kauth /=.
-  2: split_and!.
-  all: rewrite map_Forall_lookup; intros i x Hlookup;
+  { rewrite /valid_kauth map_Forall_lookup /=.
+    intros i x Hlookup. rewrite lookup_empty in Hlookup. done. }
+  repeat split;
+    rewrite map_Forall_lookup; intros i x Hlookup;
     rewrite lookup_empty in Hlookup; done.
 Qed.
 
@@ -291,11 +375,14 @@ Notation "●K a" := (kview_auth 1 a) (at level 20).
 Notation "◯K b" := (kview_frag b) (at level 20).
 
 Definition mk_meta_frag (k: KKey.t) (uid: types.UID.t) (dq: dfrac) (m: ObjectMetaV.t) : fragUR :=
-  ({[(k, uid) := (dq, to_agree (ObjectMetaV.without_resource_version m))]}, (∅, ∅)).
+  ({[(k, uid) := (dq, to_agree (ObjectMetaV.without_resource_version m))]}, (∅, (∅, ∅))).
 Definition mk_spec_frag (k: KKey.t) (uid: types.UID.t) (dq: dfrac) (s: ObjectSpecV.t) : fragUR :=
-  (∅, ({[(k, uid) := (dq, to_agree s)]}, ∅)).
+  (∅, ({[(k, uid) := (dq, to_agree s)]}, (∅, ∅))).
 Definition mk_status_frag (k: KKey.t) (uid: types.UID.t) (dq: dfrac) (s: ObjectStatusV.t) : fragUR :=
-  (∅, (∅, {[(k, uid) := (dq, to_agree s)]})).
+  (∅, (∅, ({[(k, uid) := (dq, to_agree s)]}, ∅))).
+Definition mk_reservation_frag (k: KKey.t) (status: reservation_status) : fragUR :=
+  (∅, (∅, (∅,
+    ({[k := (DfracOwn 1, to_agree status)]} : reservationUR)))).
 
 Lemma auth_valid a k obj:
   ✓ (●K a) →
@@ -537,6 +624,35 @@ Proof.
   eapply Hspec_obj; eauto.
 Qed.
 
+Lemma auth_reservation_valid a k status:
+  ✓ (●K a ⋅ ◯K (mk_reservation_frag k status)) →
+  reserved_key_pred k ∧
+  match status with
+  | Available => proj_state a !! k = None
+  | Unavailable => is_Some (proj_state a !! k)
+  end.
+Proof.
+  intros Hvalid.
+  pose proof (auth_frag_valid 0%nat a (mk_reservation_frag k status)
+    Hvalid 0%nat) as Hrel.
+  destruct Hrel as [_ [_ [_ [_ Hreservation]]]].
+  assert (Hlookup :
+    proj_reservation (mk_reservation_frag k status) !! k =
+      Some (DfracOwn 1,
+        to_agree (A := leibnizO reservation_status) status)).
+  { rewrite /proj_reservation /mk_reservation_frag /= lookup_singleton_eq //. }
+  destruct (Hreservation _ _ Hlookup) as
+    (status' & Hagree & _ & Hreserved & Hstatus_state).
+  assert (Hstatus_eqv :
+    (status : leibnizO reservation_status) ≡ status').
+  { apply (inj
+      (to_agree : leibnizO reservation_status →
+        agree (leibnizO reservation_status))).
+    exact Hagree. }
+  apply leibniz_equiv in Hstatus_eqv. subst status'.
+  done.
+Qed.
+
 Definition valid_k_uid_obj k uid obj: Prop :=
   k = KObjectV.key obj ∧
   uid = (KObjectV.objectmeta obj).(ObjectMetaV.UID') ∧
@@ -544,6 +660,7 @@ Definition valid_k_uid_obj k uid obj: Prop :=
 
 Lemma create_kobj a k uid obj:
   (proj_state a) !! k = None →
+  ¬ reserved_key_pred k →
   uid ∉ (proj_used_uid a) →
   valid_k_uid_obj k uid obj →
   no_speculative_parent_reference (KObjectV.objectmeta obj) (proj_used_uid a) →
@@ -553,11 +670,11 @@ Lemma create_kobj a k uid obj:
         ◯K (mk_spec_frag k uid 1 (KObjectV.spec obj)) ⋅
         ◯K (mk_status_frag k uid 1 (KObjectV.status obj))).
 Proof.
-  intros Hak Huid_fresh Hkuid_obj Hno_spec.
+  intros Hak Hnot_reserved Huid_fresh Hkuid_obj Hno_spec.
   destruct Hkuid_obj as (Hkey_obj & Huid_obj & Hwf_obj).
   rewrite -!assoc -!view_frag_op.
   apply view_update_alloc.
-  intros n bf [Hvalid [Hmeta [Hspec Hstatus]]].
+  intros n bf [Hvalid [Hmeta [Hspec [Hstatus Hreservation]]]].
   assert (Hmeta_bf_none : proj_meta bf !! (k, uid) = None).
   { destruct (proj_meta bf !! (k, uid)) as [[dqf agf]|] eqn:Hbf; [|done].
     exfalso.
@@ -775,7 +892,7 @@ Proof.
             ((∅ : statusUR) ⋅
               ({[(k, uid) := (DfracOwn 1, to_agree (A := leibnizO ObjectStatusV.t)
                  (KObjectV.status obj))]} : statusUR)))
-          bf.2.2 (k, uid)) in Hlookup_new.
+          bf.2.2.1 (k, uid)) in Hlookup_new.
         rewrite (lookup_op
           (∅ : statusUR)
           ((∅ : statusUR) ⋅
@@ -813,7 +930,7 @@ Proof.
               ((∅ : statusUR) ⋅
                 ({[(k, uid) := (DfracOwn 1, to_agree (A := leibnizO ObjectStatusV.t)
                    (KObjectV.status obj))]} : statusUR)))
-            bf.2.2 (k', uid')) in Hlookup_new.
+            bf.2.2.1 (k', uid')) in Hlookup_new.
           rewrite (lookup_op
             (∅ : statusUR)
             ((∅ : statusUR) ⋅
@@ -854,14 +971,458 @@ Proof.
         destruct Hlookup_obj0 as [[Hk_eq _]|[Hk_neq Hlookup_old_obj0]].
         { congruence. }
         eapply Hstatus'; done.
+    + intros k' [dq' agree_reservation'] Hlookup_new.
+      assert (Hlookup_old :
+        proj_reservation bf !! k' = Some (dq', agree_reservation')).
+      { move: Hlookup_new.
+        rewrite /proj_reservation /mk_meta_frag /mk_spec_frag
+          /mk_status_frag /kview_frag /= !left_id. done. }
+      destruct (Hreservation _ _ Hlookup_old) as
+        (reservation & Hagree & Hvdq & Hreserved & Hreservation_state).
+      exists reservation. split_and!; try done.
+      destruct reservation.
+      * assert (Hneq : k' ≠ k) by (intros ->; contradiction).
+        simpl. rewrite lookup_insert_ne //.
+      * destruct Hreservation_state as [obj' Hobj'].
+        assert (Hneq : k' ≠ k) by (intros ->; contradiction).
+        exists obj'. simpl. rewrite lookup_insert_ne //.
+Qed.
+
+Lemma create_reserved_kobj a k uid obj:
+  (proj_state a) !! k = None →
+  uid ∉ (proj_used_uid a) →
+  valid_k_uid_obj k uid obj →
+  no_speculative_parent_reference (KObjectV.objectmeta obj) (proj_used_uid a) →
+  (●K a ⋅ ◯K (mk_reservation_frag k Available)) ~~>
+    (●K ((<[k := obj]> (proj_state a)), ((proj_used_uid a) ∪ {[uid]})) ⋅
+        ◯K (mk_meta_frag k uid 1 (KObjectV.objectmeta obj)) ⋅
+        ◯K (mk_spec_frag k uid 1 (KObjectV.spec obj)) ⋅
+        ◯K (mk_status_frag k uid 1 (KObjectV.status obj)) ⋅
+        ◯K (mk_reservation_frag k Unavailable)).
+Proof.
+  intros Hak Huid_fresh Hkuid_obj Hno_spec.
+  destruct Hkuid_obj as (Hkey_obj & Huid_obj & Hwf_obj).
+  rewrite -!assoc -!view_frag_op.
+  apply view_update.
+  intros n bf [Hvalid [Hmeta [Hspec [Hstatus Hreservation]]]].
+  rewrite /proj_meta /mk_reservation_frag /= left_id in Hmeta.
+  rewrite /proj_spec /mk_reservation_frag /= left_id in Hspec.
+  rewrite /proj_status /mk_reservation_frag /= left_id in Hstatus.
+  assert (Hreservation_bf_none :
+    proj_reservation bf !! k = None).
+  { destruct (proj_reservation bf !! k) as [[dqf agf]|] eqn:Hbf;
+      last done.
+    exfalso.
+    assert (Hlookup :
+      proj_reservation (mk_reservation_frag k Available ⋅ bf) !! k =
+        Some ((DfracOwn 1,
+          to_agree (A := leibnizO reservation_status) Available) ⋅
+          (dqf, agf))).
+    { rewrite /proj_reservation /mk_reservation_frag /= lookup_op
+        lookup_singleton_eq Hbf Some_op_opM //. }
+    destruct (Hreservation _ _ Hlookup) as
+      (reservation & _ & Hvdq & _).
+    simpl in Hvdq.
+    pose proof (dfrac_valid_own_l dqf 1 Hvdq) as Hlt.
+    apply (Qp.lt_nge 1 1) in Hlt.
+    apply Hlt. done.
+  }
+  assert (Hreservation_pred : reserved_key_pred k).
+  { assert (Hlookup :
+      proj_reservation (mk_reservation_frag k Available ⋅ bf) !! k =
+        Some (DfracOwn 1,
+          to_agree (A := leibnizO reservation_status) Available)).
+    { rewrite /proj_reservation /mk_reservation_frag /= lookup_op
+        lookup_singleton_eq Hreservation_bf_none right_id //. }
+    destruct (Hreservation _ _ Hlookup) as
+      (reservation & _ & _ & Hpred & _).
+    exact Hpred.
+  }
+  assert (Htarget_meta :
+    proj_meta (mk_meta_frag k uid 1 (KObjectV.objectmeta obj) ⋅
+      (mk_spec_frag k uid 1 (KObjectV.spec obj) ⋅
+       (mk_status_frag k uid 1 (KObjectV.status obj) ⋅
+        mk_reservation_frag k Unavailable)) ⋅ bf) =
+    proj_meta (mk_meta_frag k uid 1 (KObjectV.objectmeta obj) ⋅
+      (mk_spec_frag k uid 1 (KObjectV.spec obj) ⋅
+       mk_status_frag k uid 1 (KObjectV.status obj)) ⋅ bf)).
+  { rewrite /proj_meta /mk_meta_frag /mk_spec_frag /mk_status_frag
+      /mk_reservation_frag /= !right_id. done. }
+  assert (Htarget_spec :
+    proj_spec (mk_meta_frag k uid 1 (KObjectV.objectmeta obj) ⋅
+      (mk_spec_frag k uid 1 (KObjectV.spec obj) ⋅
+       (mk_status_frag k uid 1 (KObjectV.status obj) ⋅
+        mk_reservation_frag k Unavailable)) ⋅ bf) =
+    proj_spec (mk_meta_frag k uid 1 (KObjectV.objectmeta obj) ⋅
+      (mk_spec_frag k uid 1 (KObjectV.spec obj) ⋅
+       mk_status_frag k uid 1 (KObjectV.status obj)) ⋅ bf)).
+  { rewrite /proj_spec /mk_meta_frag /mk_spec_frag /mk_status_frag
+      /mk_reservation_frag /= !left_id !right_id. done. }
+  assert (Htarget_status :
+    proj_status (mk_meta_frag k uid 1 (KObjectV.objectmeta obj) ⋅
+      (mk_spec_frag k uid 1 (KObjectV.spec obj) ⋅
+       (mk_status_frag k uid 1 (KObjectV.status obj) ⋅
+        mk_reservation_frag k Unavailable)) ⋅ bf) =
+    proj_status (mk_meta_frag k uid 1 (KObjectV.objectmeta obj) ⋅
+      (mk_spec_frag k uid 1 (KObjectV.spec obj) ⋅
+       mk_status_frag k uid 1 (KObjectV.status obj)) ⋅ bf)).
+  { rewrite /proj_status /mk_meta_frag /mk_spec_frag /mk_status_frag
+      /mk_reservation_frag /= !left_id !right_id. done. }
+  assert (Htarget_reservation :
+    proj_reservation
+      (mk_meta_frag k uid 1 (KObjectV.objectmeta obj) ⋅
+       (mk_spec_frag k uid 1 (KObjectV.spec obj) ⋅
+        (mk_status_frag k uid 1 (KObjectV.status obj) ⋅
+         mk_reservation_frag k Unavailable)) ⋅ bf) =
+    proj_reservation (mk_reservation_frag k Unavailable ⋅ bf)).
+  { rewrite /proj_reservation /mk_meta_frag /mk_spec_frag /mk_status_frag
+      /mk_reservation_frag /= !left_id. done. }
+  assert (Hmeta_bf_none : proj_meta bf !! (k, uid) = None).
+  { destruct (proj_meta bf !! (k, uid)) as [[dqf agf]|] eqn:Hbf; [|done].
+    exfalso.
+    destruct (Hmeta _ _ Hbf) as (meta0 & _ & _ & Hobj0).
+    destruct Hobj0 as (obj0 & Hlookup_obj0 & _ & _).
+    rewrite Hak in Hlookup_obj0. done.
+  }
+  assert (Hspec_bf_none : proj_spec bf !! (k, uid) = None).
+  { destruct (proj_spec bf !! (k, uid)) as [[dqf agf]|] eqn:Hbf; [|done].
+    exfalso.
+    destruct (Hspec _ _ Hbf) as (_ & _ & Huid_in & _ & _).
+    apply Huid_fresh. done.
+  }
+  assert (Hstatus_bf_none : proj_status bf !! (k, uid) = None).
+  { destruct (proj_status bf !! (k, uid)) as [[dqf agf]|] eqn:Hbf; [|done].
+    exfalso.
+    destruct (Hstatus _ _ Hbf) as (_ & _ & Huid_in & _ & _).
+    apply Huid_fresh. done.
+  }
+
+  split.
+  - eapply map_Forall_lookup_2.
+    intros k' obj' Hlookup_new.
+    destruct (decide (k' = k)) as [->|Hneq_k'].
+    + rewrite lookup_insert in Hlookup_new.
+      destruct (decide (k = k)) as [_|Hneq_k]; [|done].
+      inversion Hlookup_new. subst obj'.
+      split_and!. all: try done.
+      * rewrite Huid_obj. set_solver.
+      * intros kind name uid0 Hparent.
+        apply elem_of_union_l.
+        eapply Hno_spec. done.
+      * eapply map_Forall_lookup_2.
+        intros k'' obj'' Hlookup_new2 Huid_eq.
+        destruct (decide (k'' = k)) as [->|Hneq_k''].
+        { done. }
+        simpl in Hlookup_new2.
+        apply lookup_insert_Some in Hlookup_new2.
+        destruct Hlookup_new2 as [[Hk_eq _]|[Hk_neq Hlookup_old2]].
+        { congruence. }
+        pose proof (map_Forall_lookup_1 _ _ _ _ Hvalid Hlookup_old2) as Hkobj_old2.
+        destruct Hkobj_old2 as (_ & _ & Huid_in_old2 & _ & _).
+        exfalso.
+        apply Huid_fresh.
+        rewrite Huid_obj.
+        rewrite <- Huid_eq in Huid_in_old2.
+        done.
+    + simpl in Hlookup_new.
+      apply lookup_insert_Some in Hlookup_new.
+      destruct Hlookup_new as [[Hk_eq _]|[Hk_neq Hlookup_old]].
+      { congruence. }
+      pose proof (map_Forall_lookup_1 _ _ _ _ Hvalid Hlookup_old) as Hkobj_old.
+      destruct Hkobj_old as (Hkey_old & Hwf_old & Huid_old_in & Hno_spec_old & Huniq_old).
+      split_and!. all: try done.
+      * set_solver.
+      * intros kind name uid0 Hparent.
+        apply elem_of_union_l.
+        eapply Hno_spec_old. done.
+      * eapply map_Forall_lookup_2.
+        intros k'' obj'' Hlookup_new2 Huid_eq.
+        destruct (decide (k'' = k)) as [->|Hneq_k''].
+        { rewrite lookup_insert in Hlookup_new2.
+          destruct (decide (k = k)) as [_|Hneq_k]; [|done].
+          inversion Hlookup_new2. subst obj''.
+          exfalso.
+          apply Huid_fresh.
+          rewrite <- Huid_obj in Huid_eq.
+          rewrite Huid_eq in Huid_old_in.
+          done.
+        }
+        simpl in Hlookup_new2.
+        apply lookup_insert_Some in Hlookup_new2.
+        destruct Hlookup_new2 as [[Hk_eq2 _]|[Hk_neq2 Hlookup_old2]].
+        { congruence. }
+        eapply Huniq_old; done.
+  - split_and!.
+    + rewrite Htarget_meta.
+      intros [k' uid'] [dq' agree_meta'] Hlookup_new.
+      destruct (decide ((k', uid') = (k, uid))) as [Heq_pair|Hneq_pair].
+      * inversion Heq_pair. subst k' uid'.
+        rewrite /proj_meta /mk_meta_frag /mk_spec_frag /mk_status_frag /kview_frag /= in Hlookup_new.
+        rewrite (right_id (A := metaUR) (∅ : metaUR)) in Hlookup_new.
+	        rewrite (lookup_op
+	          (({[(k, uid) := (DfracOwn 1, to_agree (A := leibnizO ObjectMetaV.t)
+	             (ObjectMetaV.without_resource_version (KObjectV.objectmeta obj)))]} : metaUR) ⋅ ∅)
+	          bf.1 (k, uid)) in Hlookup_new.
+	        rewrite (lookup_op
+	          ({[(k, uid) := (DfracOwn 1, to_agree (A := leibnizO ObjectMetaV.t)
+	             (ObjectMetaV.without_resource_version (KObjectV.objectmeta obj)))]} : metaUR)
+	          (∅ : metaUR) (k, uid)) in Hlookup_new.
+        rewrite lookup_singleton_eq lookup_empty right_id Hmeta_bf_none right_id in Hlookup_new.
+        inversion Hlookup_new. subst dq' agree_meta'.
+	        exists (ObjectMetaV.without_resource_version (KObjectV.objectmeta obj)).
+	        split_and!. all: try done.
+        exists obj. split_and!. all: try done.
+        rewrite lookup_insert. destruct (decide (k = k)); done.
+      * assert (Hlookup_old : proj_meta bf !! (k', uid') = Some (dq', agree_meta')).
+        { rewrite /proj_meta /mk_meta_frag /mk_spec_frag /mk_status_frag /kview_frag /= in Hlookup_new.
+          rewrite (right_id (A := metaUR) (∅ : metaUR)) in Hlookup_new.
+	          assert (Hsingle_none :
+	            ({[(k, uid) := (DfracOwn 1, to_agree (A := leibnizO ObjectMetaV.t)
+	              (ObjectMetaV.without_resource_version (KObjectV.objectmeta obj)))]}
+	              : gmap (KKey.t * types.UID.t) (dfrac * agree (leibnizO ObjectMetaV.t))) !!
+	            (k', uid') = None).
+          { apply lookup_singleton_ne. done. }
+	          rewrite (lookup_op
+	            (({[(k, uid) := (DfracOwn 1, to_agree (A := leibnizO ObjectMetaV.t)
+	               (ObjectMetaV.without_resource_version (KObjectV.objectmeta obj)))]} : metaUR) ⋅ ∅)
+	            bf.1 (k', uid')) in Hlookup_new.
+	          rewrite (lookup_op
+	            ({[(k, uid) := (DfracOwn 1, to_agree (A := leibnizO ObjectMetaV.t)
+	               (ObjectMetaV.without_resource_version (KObjectV.objectmeta obj)))]} : metaUR)
+	            (∅ : metaUR) (k', uid')) in Hlookup_new.
+          rewrite Hsingle_none lookup_empty in Hlookup_new.
+          simpl in Hlookup_new.
+          rewrite (left_id
+            (A := option (dfrac * agree (leibnizO ObjectMetaV.t))) None) in Hlookup_new.
+          rewrite (left_id
+            (A := option (dfrac * agree (leibnizO ObjectMetaV.t))) None) in Hlookup_new.
+          done.
+        }
+        destruct (Hmeta _ _ Hlookup_old) as (meta' & Hagree' & Hvdq' & Hobj').
+        destruct Hobj' as (obj0 & Hlookup_obj0 & Huid_obj0 & Hmeta_obj0).
+        assert (Hneq_k : k' ≠ k).
+        { intros Hk'. subst k'.
+          rewrite Hak in Hlookup_obj0. done.
+        }
+        exists meta'. split_and!. all: try done.
+        exists obj0. split_and!. all: try done.
+        rewrite lookup_insert_ne; done.
+    + rewrite Htarget_spec.
+      intros [k' uid'] [dq' agree_spec'] Hlookup_new.
+      destruct (decide ((k', uid') = (k, uid))) as [Heq_pair|Hneq_pair].
+      * inversion Heq_pair. subst k' uid'.
+        rewrite /proj_spec /mk_meta_frag /mk_spec_frag /mk_status_frag /kview_frag /= in Hlookup_new.
+        rewrite (lookup_op
+          ((∅ : specUR) ⋅
+            (({[(k, uid) := (DfracOwn 1, to_agree (A := leibnizO ObjectSpecV.t)
+               (KObjectV.spec obj))]} : specUR) ⋅ ∅))
+          bf.2.1 (k, uid)) in Hlookup_new.
+        rewrite (lookup_op
+          (∅ : specUR)
+          (({[(k, uid) := (DfracOwn 1, to_agree (A := leibnizO ObjectSpecV.t)
+              (KObjectV.spec obj))]} : specUR) ⋅ ∅) (k, uid)) in Hlookup_new.
+        rewrite lookup_empty in Hlookup_new.
+        rewrite (left_id
+          (A := option (dfrac * agree (leibnizO ObjectSpecV.t))) None) in Hlookup_new.
+        rewrite (lookup_op
+          ({[(k, uid) := (DfracOwn 1, to_agree (A := leibnizO ObjectSpecV.t)
+             (KObjectV.spec obj))]} : specUR)
+          (∅ : specUR) (k, uid)) in Hlookup_new.
+        rewrite lookup_singleton_eq lookup_empty right_id Hspec_bf_none right_id in Hlookup_new.
+        inversion Hlookup_new. subst dq' agree_spec'.
+        exists (KObjectV.spec obj). split_and!. all: try done.
+        { rewrite Huid_obj. apply elem_of_union_r.
+          apply elem_of_singleton_2. done. }
+        intros obj0 Hlookup_obj0 Huid_obj0.
+        rewrite lookup_insert in Hlookup_obj0.
+        destruct (decide (k = k)) as [_|Hneq_k]; [|done].
+        inversion Hlookup_obj0. subst obj0. done.
+      * assert (Hlookup_old : proj_spec bf !! (k', uid') = Some (dq', agree_spec')).
+        { rewrite /proj_spec /mk_meta_frag /mk_spec_frag /mk_status_frag /kview_frag /= in Hlookup_new.
+          assert (Hsingle_none :
+            ({[(k, uid) := (DfracOwn 1, to_agree (A := leibnizO ObjectSpecV.t)
+              (KObjectV.spec obj))]}
+              : gmap (KKey.t * types.UID.t) (dfrac * agree (leibnizO ObjectSpecV.t))) !!
+            (k', uid') = None).
+          { apply lookup_singleton_ne. done. }
+          rewrite (lookup_op
+            ((∅ : specUR) ⋅
+              (({[(k, uid) := (DfracOwn 1, to_agree (A := leibnizO ObjectSpecV.t)
+                 (KObjectV.spec obj))]} : specUR) ⋅ ∅))
+            bf.2.1 (k', uid')) in Hlookup_new.
+          rewrite (lookup_op
+            (∅ : specUR)
+            (({[(k, uid) := (DfracOwn 1, to_agree (A := leibnizO ObjectSpecV.t)
+                (KObjectV.spec obj))]} : specUR) ⋅ ∅) (k', uid')) in Hlookup_new.
+          rewrite lookup_empty in Hlookup_new.
+          rewrite (left_id
+            (A := option (dfrac * agree (leibnizO ObjectSpecV.t))) None) in Hlookup_new.
+          rewrite (lookup_op
+            ({[(k, uid) := (DfracOwn 1, to_agree (A := leibnizO ObjectSpecV.t)
+               (KObjectV.spec obj))]} : specUR)
+            (∅ : specUR) (k', uid')) in Hlookup_new.
+          rewrite Hsingle_none lookup_empty in Hlookup_new.
+          simpl in Hlookup_new.
+          rewrite (left_id
+            (A := option (dfrac * agree (leibnizO ObjectSpecV.t))) None) in Hlookup_new.
+          rewrite (left_id
+            (A := option (dfrac * agree (leibnizO ObjectSpecV.t))) None) in Hlookup_new.
+          done.
+        }
+        destruct (Hspec _ _ Hlookup_old) as (spec' & Hagree' & Huid_in' & Hvdq' & Hspec').
+        exists spec'. split_and!. all: try done.
+        { apply elem_of_union_l. done. }
+        intros obj0 Hlookup_obj0 Huid_obj0.
+        destruct (decide (k' = k)) as [->|Hneq_k'].
+        { rewrite lookup_insert in Hlookup_obj0.
+          destruct (decide (k = k)) as [_|Hneq_k]; [|done].
+          inversion Hlookup_obj0. subst obj0.
+          exfalso.
+          apply Hneq_pair.
+          rewrite <- Huid_obj in Huid_obj0.
+          congruence.
+        }
+        simpl in Hlookup_obj0.
+        apply lookup_insert_Some in Hlookup_obj0.
+        destruct Hlookup_obj0 as [[Hk_eq _]|[Hk_neq Hlookup_old_obj0]].
+        { congruence. }
+        eapply Hspec'; done.
+    + rewrite Htarget_status.
+      intros [k' uid'] [dq' agree_status'] Hlookup_new.
+      destruct (decide ((k', uid') = (k, uid))) as [Heq_pair|Hneq_pair].
+      * inversion Heq_pair. subst k' uid'.
+        rewrite /proj_status /mk_meta_frag /mk_spec_frag /mk_status_frag /kview_frag /= in Hlookup_new.
+        rewrite (lookup_op
+          ((∅ : statusUR) ⋅
+            ((∅ : statusUR) ⋅
+              ({[(k, uid) := (DfracOwn 1, to_agree (A := leibnizO ObjectStatusV.t)
+                 (KObjectV.status obj))]} : statusUR)))
+          bf.2.2.1 (k, uid)) in Hlookup_new.
+        rewrite (lookup_op
+          (∅ : statusUR)
+          ((∅ : statusUR) ⋅
+            ({[(k, uid) := (DfracOwn 1, to_agree (A := leibnizO ObjectStatusV.t)
+               (KObjectV.status obj))]} : statusUR)) (k, uid)) in Hlookup_new.
+        rewrite lookup_empty in Hlookup_new.
+        rewrite (left_id
+          (A := option (dfrac * agree (leibnizO ObjectStatusV.t))) None) in Hlookup_new.
+        rewrite (lookup_op
+          (∅ : statusUR)
+          ({[(k, uid) := (DfracOwn 1, to_agree (A := leibnizO ObjectStatusV.t)
+             (KObjectV.status obj))]} : statusUR) (k, uid)) in Hlookup_new.
+        rewrite lookup_empty in Hlookup_new.
+        rewrite (left_id
+          (A := option (dfrac * agree (leibnizO ObjectStatusV.t))) None) in Hlookup_new.
+        rewrite lookup_singleton_eq Hstatus_bf_none right_id in Hlookup_new.
+        inversion Hlookup_new. subst dq' agree_status'.
+        exists (KObjectV.status obj). split_and!. all: try done.
+        { rewrite Huid_obj. apply elem_of_union_r.
+          apply elem_of_singleton_2. reflexivity. }
+        intros obj0 Hlookup_obj0 Huid_obj0.
+        rewrite lookup_insert in Hlookup_obj0.
+        destruct (decide (k = k)) as [_|Hneq_k]; [|done].
+        inversion Hlookup_obj0. subst obj0. done.
+      * assert (Hlookup_old : proj_status bf !! (k', uid') = Some (dq', agree_status')).
+        { rewrite /proj_status /mk_meta_frag /mk_spec_frag /mk_status_frag /kview_frag /= in Hlookup_new.
+          assert (Hsingle_none :
+            ({[(k, uid) := (DfracOwn 1, to_agree (A := leibnizO ObjectStatusV.t)
+              (KObjectV.status obj))]}
+              : gmap (KKey.t * types.UID.t) (dfrac * agree (leibnizO ObjectStatusV.t))) !!
+            (k', uid') = None).
+          { apply lookup_singleton_ne. done. }
+          rewrite (lookup_op
+            ((∅ : statusUR) ⋅
+              ((∅ : statusUR) ⋅
+                ({[(k, uid) := (DfracOwn 1, to_agree (A := leibnizO ObjectStatusV.t)
+                   (KObjectV.status obj))]} : statusUR)))
+            bf.2.2.1 (k', uid')) in Hlookup_new.
+          rewrite (lookup_op
+            (∅ : statusUR)
+            ((∅ : statusUR) ⋅
+              ({[(k, uid) := (DfracOwn 1, to_agree (A := leibnizO ObjectStatusV.t)
+                 (KObjectV.status obj))]} : statusUR)) (k', uid')) in Hlookup_new.
+          rewrite lookup_empty in Hlookup_new.
+          rewrite (left_id
+            (A := option (dfrac * agree (leibnizO ObjectStatusV.t))) None) in Hlookup_new.
+          rewrite (lookup_op
+            (∅ : statusUR)
+            ({[(k, uid) := (DfracOwn 1, to_agree (A := leibnizO ObjectStatusV.t)
+               (KObjectV.status obj))]} : statusUR) (k', uid')) in Hlookup_new.
+          rewrite lookup_empty in Hlookup_new.
+          rewrite (left_id
+            (A := option (dfrac * agree (leibnizO ObjectStatusV.t))) None) in Hlookup_new.
+          rewrite Hsingle_none in Hlookup_new.
+          simpl in Hlookup_new.
+          rewrite (left_id
+            (A := option (dfrac * agree (leibnizO ObjectStatusV.t))) None) in Hlookup_new.
+          done.
+        }
+        destruct (Hstatus _ _ Hlookup_old) as
+          (status' & Hagree' & Huid_in' & Hvdq' & Hstatus').
+        exists status'. split_and!. all: try done.
+        { apply elem_of_union_l. exact Huid_in'. }
+        intros obj0 Hlookup_obj0 Huid_obj0.
+        destruct (decide (k' = k)) as [->|Hneq_k'].
+        { rewrite lookup_insert in Hlookup_obj0.
+          destruct (decide (k = k)) as [_|Hneq_k]; [|done].
+          inversion Hlookup_obj0. subst obj0.
+          exfalso.
+          apply Hneq_pair.
+          rewrite <- Huid_obj in Huid_obj0.
+          congruence.
+        }
+        simpl in Hlookup_obj0.
+        apply lookup_insert_Some in Hlookup_obj0.
+        destruct Hlookup_obj0 as [[Hk_eq _]|[Hk_neq Hlookup_old_obj0]].
+        { congruence. }
+        eapply Hstatus'; done.
+    + intros k' [dq' agree_reservation'] Hlookup_new.
+      destruct (decide (k' = k)) as [->|Hneq].
+      * assert (Hlookup_target :
+          proj_reservation (mk_reservation_frag k Unavailable ⋅ bf) !! k =
+          Some (DfracOwn 1,
+            to_agree (A := leibnizO reservation_status) Unavailable)).
+        { rewrite /proj_reservation /mk_reservation_frag /= lookup_op
+            lookup_singleton_eq
+            Hreservation_bf_none right_id //. }
+        rewrite Htarget_reservation in Hlookup_new.
+        rewrite Hlookup_target in Hlookup_new.
+        inversion Hlookup_new. subst dq' agree_reservation'.
+        exists Unavailable. split_and!; try done.
+        exists obj. simpl. rewrite lookup_insert_eq. done.
+      * assert (Hlookup_bf :
+          proj_reservation bf !! k' = Some (dq', agree_reservation')).
+        { assert (Hneq' : k ≠ k') by (intros ->; apply Hneq; done).
+          rewrite Htarget_reservation in Hlookup_new.
+          rewrite /proj_reservation /mk_reservation_frag /= lookup_op
+            lookup_singleton_ne // left_id in Hlookup_new.
+          exact Hlookup_new. }
+        assert (Hlookup_old :
+          proj_reservation (mk_reservation_frag k Available ⋅ bf) !! k' =
+            Some (dq', agree_reservation')).
+        { assert (Hneq' : k ≠ k') by (intros ->; apply Hneq; done).
+          rewrite /proj_reservation /mk_reservation_frag /= lookup_op.
+          rewrite lookup_singleton_ne //.
+          rewrite Hlookup_bf left_id //. }
+        destruct (Hreservation _ _ Hlookup_old) as
+          (reservation & Hagree & Hvdq & Hreserved & Hreservation_state).
+        exists reservation. split_and!; try done.
+        destruct reservation.
+        { simpl. rewrite lookup_insert_ne //.
+        }
+        { destruct Hreservation_state as [obj' Hobj'].
+          exists obj'. simpl. rewrite lookup_insert_ne //.
+        }
 Qed.
 
 Lemma delete_kobj a k uid meta:
+  ¬ reserved_key_pred k →
   ●K a ⋅ ◯K (mk_meta_frag k uid 1 meta) ~~>
     ●K (delete k (proj_state a), proj_used_uid a).
 Proof.
+  intros Hnot_reserved.
   apply view_update_dealloc.
-  intros n bf [Hvalid [Hmeta [Hspec Hstatus]]].
+  intros n bf [Hvalid [Hmeta [Hspec [Hstatus Hreservation]]]].
   assert (Hbf_none : proj_meta bf !! (k, uid) = None).
   { destruct (proj_meta bf !! (k, uid)) as [[dqf agf]|] eqn:Hbf; [|done].
     exfalso.
@@ -964,6 +1525,232 @@ Proof.
       simpl in Hlookup.
       apply lookup_delete_Some in Hlookup as [_ Hlookup].
       eapply Hstatus'; done.
+    + intros k' [dq' agree_reservation'] Hlookup_bf.
+      assert (Hlookup_old :
+        (proj_reservation (mk_meta_frag k uid 1 meta ⋅ bf)) !! k' =
+          Some (dq', agree_reservation')).
+      { rewrite /proj_reservation /mk_meta_frag /= lookup_op lookup_empty
+          left_id. done. }
+      destruct (Hreservation _ _ Hlookup_old) as
+        (reservation & Hagree & Hvdq & Hreserved & Hreservation_state).
+      exists reservation. split_and!; try done.
+      assert (Hneq : k' ≠ k) by (intros ->; contradiction).
+      destruct reservation.
+      * simpl. rewrite lookup_delete_ne //.
+      * destruct Hreservation_state as [obj' Hobj'].
+        exists obj'. simpl. rewrite lookup_delete_ne //.
+Qed.
+
+Lemma delete_reserved_kobj a k uid meta:
+  (●K a ⋅ ◯K (mk_meta_frag k uid 1 meta) ⋅
+    ◯K (mk_reservation_frag k Unavailable)) ~~>
+    (●K (delete k (proj_state a), proj_used_uid a) ⋅
+      ◯K (mk_reservation_frag k Available)).
+Proof.
+  rewrite -!assoc -!view_frag_op.
+  apply view_update.
+  intros n bf [Hvalid [Hmeta [Hspec [Hstatus Hreservation]]]].
+  assert (Hsource_meta :
+    proj_meta ((mk_meta_frag k uid 1 meta ⋅
+      mk_reservation_frag k Unavailable) ⋅ bf) =
+    proj_meta (mk_meta_frag k uid 1 meta ⋅ bf)).
+  { rewrite /proj_meta /mk_meta_frag /mk_reservation_frag /= !right_id.
+    done. }
+  assert (Hsource_spec :
+    proj_spec ((mk_meta_frag k uid 1 meta ⋅
+      mk_reservation_frag k Unavailable) ⋅ bf) =
+    proj_spec (mk_meta_frag k uid 1 meta ⋅ bf)).
+  { rewrite /proj_spec /mk_meta_frag /mk_reservation_frag /= !left_id.
+    done. }
+  assert (Hsource_status :
+    proj_status ((mk_meta_frag k uid 1 meta ⋅
+      mk_reservation_frag k Unavailable) ⋅ bf) =
+    proj_status (mk_meta_frag k uid 1 meta ⋅ bf)).
+  { rewrite /proj_status /mk_meta_frag /mk_reservation_frag /= !left_id.
+    done. }
+  rewrite Hsource_meta in Hmeta.
+  rewrite Hsource_spec in Hspec.
+  rewrite Hsource_status in Hstatus.
+  assert (Hreservation_bf_none :
+    proj_reservation bf !! k = None).
+  { destruct (proj_reservation bf !! k) as [[dqf agf]|] eqn:Hbf;
+      last done.
+    exfalso.
+    assert (Hlookup :
+      proj_reservation ((mk_meta_frag k uid 1 meta ⋅
+        mk_reservation_frag k Unavailable) ⋅ bf) !! k =
+        Some ((DfracOwn 1,
+          to_agree (A := leibnizO reservation_status) Unavailable) ⋅
+          (dqf, agf))).
+    { rewrite /proj_reservation /mk_meta_frag /mk_reservation_frag /=
+        !lookup_op !lookup_empty !left_id lookup_singleton_eq Hbf
+        Some_op_opM //. }
+    destruct (Hreservation _ _ Hlookup) as
+      (reservation & _ & Hvdq & _).
+    simpl in Hvdq.
+    pose proof (dfrac_valid_own_l dqf 1 Hvdq) as Hlt.
+    apply (Qp.lt_nge 1 1) in Hlt.
+    apply Hlt. done.
+  }
+  assert (Hreservation_pred : reserved_key_pred k).
+  { assert (Hlookup :
+      proj_reservation ((mk_meta_frag k uid 1 meta ⋅
+        mk_reservation_frag k Unavailable) ⋅ bf) !! k =
+        Some (DfracOwn 1,
+          to_agree (A := leibnizO reservation_status) Unavailable)).
+    { rewrite /proj_reservation /mk_meta_frag /mk_reservation_frag /=
+        !lookup_op !lookup_empty !left_id lookup_singleton_eq
+        Hreservation_bf_none right_id //. }
+    destruct (Hreservation _ _ Hlookup) as
+      (reservation & _ & _ & Hpred & _).
+    exact Hpred.
+  }
+  assert (Htarget_meta :
+    proj_meta (mk_reservation_frag k Available ⋅ bf) = proj_meta bf).
+  { rewrite /proj_meta /mk_reservation_frag /= left_id //. }
+  assert (Htarget_spec :
+    proj_spec (mk_reservation_frag k Available ⋅ bf) = proj_spec bf).
+  { rewrite /proj_spec /mk_reservation_frag /= left_id //. }
+  assert (Htarget_status :
+    proj_status (mk_reservation_frag k Available ⋅ bf) = proj_status bf).
+  { rewrite /proj_status /mk_reservation_frag /= left_id //. }
+  assert (Hbf_none : proj_meta bf !! (k, uid) = None).
+  { destruct (proj_meta bf !! (k, uid)) as [[dqf agf]|] eqn:Hbf; [|done].
+    exfalso.
+	    assert (Hlookup :
+	      (proj_meta (mk_meta_frag k uid 1 meta ⋅ bf)) !! (k, uid) =
+	      Some ((DfracOwn 1, to_agree (A := leibnizO ObjectMetaV.t)
+	        (ObjectMetaV.without_resource_version meta)) ⋅ (dqf, agf))).
+    { rewrite /proj_meta /mk_meta_frag /= lookup_op.
+      rewrite lookup_singleton_eq Hbf Some_op_opM //. }
+    destruct (Hmeta _ _ Hlookup) as (meta0 & _ & Hvdq & _).
+    simpl in Hvdq.
+    pose proof (dfrac_valid_own_l dqf 1 Hvdq) as Hlt.
+    apply (Qp.lt_nge 1 1) in Hlt.
+    apply Hlt. done.
+  }
+	  assert (Hlookup_k :
+	    (proj_meta (mk_meta_frag k uid 1 meta ⋅ bf)) !! (k, uid) =
+	    Some (DfracOwn 1, to_agree (A := leibnizO ObjectMetaV.t)
+	      (ObjectMetaV.without_resource_version meta))).
+  { rewrite /proj_meta /mk_meta_frag /= lookup_op.
+    rewrite lookup_singleton_eq Hbf_none right_id //. }
+  destruct (Hmeta _ _ Hlookup_k) as (meta0 & Hagree0 & _ & Hobj0).
+  destruct Hobj0 as (obj0 & Hobj0_lookup & Hobj0_uid & Hobj0_meta).
+	  assert (Hmeta_eqv : (ObjectMetaV.without_resource_version meta : leibnizO ObjectMetaV.t) ≡ meta0).
+  { apply (inj (to_agree : leibnizO ObjectMetaV.t → agree (leibnizO ObjectMetaV.t))).
+    by rewrite Hagree0.
+  }
+  apply leibniz_equiv in Hmeta_eqv. subst meta0.
+  assert (Hbf_none_obj0 :
+    proj_meta bf !! (k, ObjectMetaV.UID' (KObjectV.objectmeta obj0)) = None).
+  { rewrite Hobj0_uid. done. }
+
+  split.
+  - intros k' obj' Hlookup.
+    simpl in Hlookup.
+    apply lookup_delete_Some in Hlookup as [_ Hlookup].
+    pose proof (map_Forall_lookup_1 _ _ _ _ Hvalid Hlookup) as Hkobj.
+    destruct Hkobj as (Hkey & Hwf & Huid_in & Hno_spec & Huniq).
+    split_and!. all: try done.
+    apply map_Forall_delete. done.
+  - split_and!.
+    + rewrite Htarget_meta.
+      intros [k' uid'] [dq' agree_meta'] Hlookup_bf.
+      assert (Hneq_pair : (k', uid') ≠ (k, uid)).
+      { intros Heq. inversion Heq. subst.
+        rewrite Hbf_none_obj0 in Hlookup_bf. done.
+      }
+      assert (Hlookup_old :
+        (proj_meta (mk_meta_frag k uid 1 meta ⋅ bf)) !! (k', uid') =
+        Some (dq', agree_meta')).
+      { rewrite /proj_meta /mk_meta_frag /=.
+	        rewrite (lookup_op
+	          ({[(k, uid) := (DfracOwn 1, to_agree (A := leibnizO ObjectMetaV.t)
+	            (ObjectMetaV.without_resource_version meta))]})
+	          (proj_meta bf) (k', uid')).
+	        assert (Hsingle_none :
+	          (({[(k, uid) := (DfracOwn 1, to_agree (A := leibnizO ObjectMetaV.t)
+	            (ObjectMetaV.without_resource_version meta))]}
+	            : gmap (KKey.t * types.UID.t) (dfrac * agree (leibnizO ObjectMetaV.t))) !!
+            (k', uid')) = None).
+        { apply lookup_singleton_ne. done. }
+        rewrite Hsingle_none.
+        rewrite Hlookup_bf left_id //. }
+      destruct (Hmeta _ _ Hlookup_old) as (meta' & Hagree' & Hvdq' & Hobj').
+      destruct Hobj' as (obj' & Hobj'_lookup & Hobj'_uid & Hobj'_meta).
+      assert (Hneq_k : k' ≠ k).
+      { intros Hk'. subst k'.
+        rewrite Hobj0_lookup in Hobj'_lookup. inversion Hobj'_lookup. subst obj'.
+        assert (Huid' : uid' = uid) by congruence.
+        subst uid'. exfalso. apply Hneq_pair.
+        apply (f_equal (λ u, (k, u))). done.
+      }
+      exists meta'.
+      split_and!. all: try done.
+      exists obj'. split_and!. all: try done.
+      apply lookup_delete_Some. split; [done|done].
+    + rewrite Htarget_spec.
+      intros [k' uid'] [dq' agree_spec'] Hlookup_bf.
+      assert (Hlookup_old :
+        (proj_spec (mk_meta_frag k uid 1 meta ⋅ bf)) !! (k', uid') =
+        Some (dq', agree_spec')).
+      { rewrite /proj_spec /mk_meta_frag /=.
+        rewrite (lookup_op ∅ (proj_spec bf) (k', uid')).
+        rewrite lookup_empty left_id. done. }
+      destruct (Hspec _ _ Hlookup_old) as (spec' & Hagree' & Huid' & Hvdq' & Hspec').
+      exists spec'. split_and!. all: try done.
+      intros obj Hlookup Huid_obj.
+      simpl in Hlookup.
+      apply lookup_delete_Some in Hlookup as [_ Hlookup].
+      eapply Hspec'; done.
+    + rewrite Htarget_status.
+      intros [k' uid'] [dq' agree_status'] Hlookup_bf.
+      assert (Hlookup_old :
+        (proj_status (mk_meta_frag k uid 1 meta ⋅ bf)) !! (k', uid') =
+        Some (dq', agree_status')).
+      { rewrite /proj_status /mk_meta_frag /=.
+        rewrite (lookup_op ∅ (proj_status bf) (k', uid')).
+        rewrite lookup_empty left_id. done. }
+      destruct (Hstatus _ _ Hlookup_old) as
+        (status' & Hagree' & Huid' & Hvdq' & Hstatus').
+      exists status'. split_and!. all: try done.
+      intros obj Hlookup Huid_obj.
+      simpl in Hlookup.
+      apply lookup_delete_Some in Hlookup as [_ Hlookup].
+      eapply Hstatus'; done.
+    + intros k' [dq' agree_reservation'] Hlookup_new.
+      destruct (decide (k' = k)) as [->|Hneq].
+      * assert (Hlookup_target :
+          proj_reservation (mk_reservation_frag k Available ⋅ bf) !! k =
+          Some (DfracOwn 1,
+            to_agree (A := leibnizO reservation_status) Available)).
+        { rewrite /proj_reservation /mk_reservation_frag /= lookup_op
+            lookup_singleton_eq Hreservation_bf_none right_id //. }
+        rewrite Hlookup_target in Hlookup_new.
+        inversion Hlookup_new. subst dq' agree_reservation'.
+        exists Available. split_and!; try done.
+        simpl. apply lookup_delete_eq.
+      * assert (Hneq' : k ≠ k') by (intros ->; apply Hneq; done).
+        assert (Hlookup_bf :
+          proj_reservation bf !! k' = Some (dq', agree_reservation')).
+        { rewrite /proj_reservation /mk_reservation_frag /= lookup_op
+            lookup_singleton_ne // left_id in Hlookup_new.
+          exact Hlookup_new. }
+        assert (Hlookup_old :
+          proj_reservation ((mk_meta_frag k uid 1 meta ⋅
+            mk_reservation_frag k Unavailable) ⋅ bf) !! k' =
+            Some (dq', agree_reservation')).
+        { rewrite /proj_reservation /mk_meta_frag /mk_reservation_frag /=
+            !lookup_op !lookup_empty !left_id lookup_singleton_ne //
+            Hlookup_bf left_id //. }
+        destruct (Hreservation _ _ Hlookup_old) as
+          (reservation & Hagree & Hvdq & Hreserved & Hreservation_state).
+        exists reservation. split_and!; try done.
+        destruct reservation.
+        { simpl. rewrite lookup_delete_ne //. }
+        { destruct Hreservation_state as [obj' Hobj'].
+          exists obj'. simpl. rewrite lookup_delete_ne //. }
 Qed.
 
 Lemma update_meta_kobj a k uid meta prev_obj obj:
@@ -979,7 +1766,7 @@ Proof.
   intros Hkuid_obj Hno_spec Hak Hspec_eq Hstatus_eq.
   destruct Hkuid_obj as (Hkey_obj & Huid_obj & Hwf_obj).
   apply view_update.
-  intros n bf [Hvalid [Hmeta [Hspec Hstatus]]].
+  intros n bf [Hvalid [Hmeta [Hspec [Hstatus Hreservation]]]].
   assert (Hmeta_bf_none : proj_meta bf !! (k, uid) = None).
   { destruct (proj_meta bf !! (k, uid)) as [[dqf agf]|] eqn:Hbf; [|done].
     exfalso.
@@ -1179,6 +1966,23 @@ Proof.
         destruct Hlookup_obj0 as [[Hk_eq _]|[Hk_neq Hlookup_old_obj0]].
         { congruence. }
         eapply Hstatus'; done.
+    + intros k' [dq' agree_reservation'] Hlookup_new.
+      assert (Hlookup_old :
+        proj_reservation (mk_meta_frag k uid 1 meta ⋅ bf) !! k' =
+          Some (dq', agree_reservation')).
+      { move: Hlookup_new.
+        rewrite /proj_reservation /mk_meta_frag /= !left_id. done. }
+      destruct (Hreservation _ _ Hlookup_old) as
+        (reservation & Hagree & Hvdq & Hreserved & Hreservation_state).
+      exists reservation. split_and!; try done.
+      destruct reservation.
+      * assert (Hneq : k' ≠ k).
+        { intros ->. rewrite Hak in Hreservation_state. done. }
+        simpl. rewrite lookup_insert_ne //.
+      * destruct Hreservation_state as [obj' Hobj'].
+        destruct (decide (k' = k)) as [->|Hneq].
+        { exists obj. simpl. rewrite lookup_insert_eq. done. }
+        { exists obj'. simpl. rewrite lookup_insert_ne //. }
 Qed.
 
 Lemma update_kobj a k uid meta spec prev_obj obj:
@@ -1197,7 +2001,7 @@ Proof.
   destruct Hkuid_obj as (Hkey_obj & Huid_obj & Hwf_obj).
   rewrite -!assoc -!view_frag_op.
   apply view_update.
-  intros n bf [Hvalid [Hmeta [Hspec Hstatus]]].
+  intros n bf [Hvalid [Hmeta [Hspec [Hstatus Hreservation]]]].
   assert (Hmeta_bf_none : proj_meta bf !! (k, uid) = None).
   { destruct (proj_meta bf !! (k, uid)) as [[dqf agf]|] eqn:Hbf; [|done].
     exfalso.
@@ -1460,6 +2264,25 @@ Proof.
         destruct Hlookup_obj0 as [[Hk_eq _]|[Hk_neq Hlookup_old_obj0]].
         { congruence. }
         eapply Hstatus'; done.
+    + intros k' [dq' agree_reservation'] Hlookup_new.
+      assert (Hlookup_old :
+        proj_reservation (mk_meta_frag k uid 1 meta ⋅
+          mk_spec_frag k uid 1 spec ⋅ bf) !! k' =
+          Some (dq', agree_reservation')).
+      { move: Hlookup_new.
+        rewrite /proj_reservation /mk_meta_frag /mk_spec_frag /= !left_id.
+        done. }
+      destruct (Hreservation _ _ Hlookup_old) as
+        (reservation & Hagree & Hvdq & Hreserved & Hreservation_state).
+      exists reservation. split_and!; try done.
+      destruct reservation.
+      * assert (Hneq : k' ≠ k).
+        { intros ->. rewrite Hak in Hreservation_state. done. }
+        simpl. rewrite lookup_insert_ne //.
+      * destruct Hreservation_state as [obj' Hobj'].
+        destruct (decide (k' = k)) as [->|Hneq].
+        { exists obj. simpl. rewrite lookup_insert_eq. done. }
+        { exists obj'. simpl. rewrite lookup_insert_ne //. }
 Qed.
 
 Lemma update_status_kobj a k uid meta status prev_obj obj:
@@ -1478,7 +2301,7 @@ Proof.
   destruct Hkuid_obj as (Hkey_obj & Huid_obj & Hwf_obj).
   rewrite -!assoc -!view_frag_op.
   apply view_update.
-  intros n bf [Hvalid [Hmeta [Hspec Hstatus]]].
+  intros n bf [Hvalid [Hmeta [Hspec [Hstatus Hreservation]]]].
   assert (Hmeta_bf_none : proj_meta bf !! (k, uid) = None).
   { destruct (proj_meta bf !! (k, uid)) as [[dqf agf]|] eqn:Hbf; [|done].
     exfalso.
@@ -1742,6 +2565,25 @@ Proof.
         destruct Hlookup_obj0 as [[Hk_eq _]|[Hk_neq Hlookup_old_obj0]].
         { congruence. }
         eapply Hstatus'; done.
+    + intros k' [dq' agree_reservation'] Hlookup_new.
+      assert (Hlookup_old :
+        proj_reservation (mk_meta_frag k uid 1 meta ⋅
+          mk_status_frag k uid 1 status ⋅ bf) !! k' =
+          Some (dq', agree_reservation')).
+      { move: Hlookup_new.
+        rewrite /proj_reservation /mk_meta_frag /mk_status_frag /= !left_id.
+        done. }
+      destruct (Hreservation _ _ Hlookup_old) as
+        (reservation & Hagree & Hvdq & Hreserved & Hreservation_state).
+      exists reservation. split_and!; try done.
+      destruct reservation.
+      * assert (Hneq : k' ≠ k).
+        { intros ->. rewrite Hak in Hreservation_state. done. }
+        simpl. rewrite lookup_insert_ne //.
+      * destruct Hreservation_state as [obj' Hobj'].
+        destruct (decide (k' = k)) as [->|Hneq].
+        { exists obj. simpl. rewrite lookup_insert_eq. done. }
+        { exists obj'. simpl. rewrite lookup_insert_ne //. }
 Qed.
 
 Class kviewG Σ :=
@@ -1774,6 +2616,9 @@ Definition own_spec_frag γ k uid dq sp : iProp Σ :=
 
 Definition own_status_frag γ k uid dq st : iProp Σ :=
   own γ (◯K (mk_status_frag k uid dq st)).
+
+Definition own_reservation_frag γ k status : iProp Σ :=
+  own γ (◯K (mk_reservation_frag k status)).
 
 Lemma own_auth_valid {γ state used_uid} k obj:
   own_auth γ state used_uid -∗
@@ -1853,6 +2698,32 @@ Proof.
     exact Hrel0.
   }
   exact (auth_valid_forall (state, used_uid) Hvalid).
+Qed.
+
+Lemma own_reservation_valid {γ state used_uid k status}:
+  own_auth γ state used_uid -∗
+  own_reservation_frag γ k status -∗
+  ⌜ reserved_key_pred k ∧
+    match status with
+    | Available => state !! k = None
+    | Unavailable => is_Some (state !! k)
+    end ⌝.
+Proof.
+  iIntros "Hauth Hreservation".
+  iDestruct (own_valid_2 with "Hauth Hreservation") as "Hvalid".
+  iDestruct (internal_cmra_valid_elim with "Hvalid") as %Hvalid0.
+  iPureIntro.
+  rewrite /own_auth /own_reservation_frag /kview_auth /kview_frag in Hvalid0.
+  pose proof (proj1 (view_both_validN view_rel 0%nat
+    (state, used_uid) (mk_reservation_frag k status)) Hvalid0) as Hrel0.
+  assert (Hvalid :
+    ✓ (●K (state, used_uid) ⋅ ◯K (mk_reservation_frag k status))).
+  { rewrite /kview_auth /kview_frag.
+    apply (proj2 (view_both_valid view_rel
+      (state, used_uid) (mk_reservation_frag k status))).
+    intros n. exact Hrel0. }
+  apply (auth_reservation_valid (state, used_uid) k status).
+  exact Hvalid.
 Qed.
 
 Lemma own_meta_valid {γ k uid dq meta}:
@@ -2203,7 +3074,7 @@ Proof.
   intros obj Hlookup_obj Huid_obj.
   pose proof (auth_frag_valid 0%nat (state, used_uid) (mk_status_frag k uid dq status) Hvalid 0%nat)
     as Hrel.
-  destruct Hrel as [_ [_ [_ Hstatus]]].
+  destruct Hrel as [_ [_ [_ [Hstatus _]]]].
   assert (Hlookup :
     proj_status (mk_status_frag k uid dq status) !! (k, uid) =
     Some (dq, to_agree (A := leibnizO ObjectStatusV.t) status)).
@@ -2220,6 +3091,7 @@ Qed.
 
 Lemma create_kobj_vs {γ state used_uid} k uid obj:
   state !! k = None →
+  ¬ reserved_key_pred k →
   uid ∉ used_uid →
   valid_k_uid_obj k uid obj →
   no_speculative_parent_reference (KObjectV.objectmeta obj) used_uid →
@@ -2229,7 +3101,7 @@ Lemma create_kobj_vs {γ state used_uid} k uid obj:
     own_spec_frag γ k uid 1 (KObjectV.spec obj) ∗
     own_status_frag γ k uid 1 (KObjectV.status obj).
 Proof.
-  iIntros (Hak Hfresh Hkuid_obj Hno_spec) "Hauth".
+  iIntros (Hak Hnot_reserved Hfresh Hkuid_obj Hno_spec) "Hauth".
   iMod (own_update with "Hauth") as "H".
   { eapply create_kobj; done. }
   iModIntro.
@@ -2239,14 +3111,54 @@ Proof.
   iFrame.
 Qed.
 
+Lemma create_reserved_kobj_vs {γ state used_uid} k uid obj:
+  state !! k = None →
+  uid ∉ used_uid →
+  valid_k_uid_obj k uid obj →
+  no_speculative_parent_reference (KObjectV.objectmeta obj) used_uid →
+  own_auth γ state used_uid -∗
+  own_reservation_frag γ k Available ==∗
+    own_auth γ (<[k := obj]> state) (used_uid ∪ {[uid]}) ∗
+    own_meta_frag γ k uid 1 (KObjectV.objectmeta obj) ∗
+    own_spec_frag γ k uid 1 (KObjectV.spec obj) ∗
+    own_status_frag γ k uid 1 (KObjectV.status obj) ∗
+    own_reservation_frag γ k Unavailable.
+Proof.
+  iIntros (Hak Hfresh Hkuid_obj Hno_spec) "Hauth Hreservation".
+  iMod (own_update_2 with "Hauth Hreservation") as "H".
+  { eapply create_reserved_kobj; done. }
+  iModIntro.
+  iDestruct (own_op with "H") as "[H Hreservation]".
+  iDestruct (own_op with "H") as "[H Hstatus]".
+  iDestruct (own_op with "H") as "[H Hspec]".
+  iDestruct (own_op with "H") as "[Hauth Hmeta]".
+  iFrame.
+Qed.
+
 Lemma delete_kobj_vs {γ state used_uid k uid meta}:
+  ¬ reserved_key_pred k →
   own_auth γ state used_uid -∗ own_meta_frag γ k uid 1 meta ==∗
     own_auth γ (delete k state) used_uid.
 Proof.
-  iIntros "Hauth Hmeta".
+  iIntros (Hnot_reserved) "Hauth Hmeta".
   iMod (own_update_2 with "Hauth Hmeta") as "Hauth".
   { eapply delete_kobj; done. }
   iModIntro. done.
+Qed.
+
+Lemma delete_reserved_kobj_vs {γ state used_uid k uid meta}:
+  own_auth γ state used_uid -∗
+  own_meta_frag γ k uid 1 meta -∗
+  own_reservation_frag γ k Unavailable ==∗
+    own_auth γ (delete k state) used_uid ∗
+    own_reservation_frag γ k Available.
+Proof.
+  iIntros "Hauth Hmeta Hreservation".
+  iMod (own_update_3 with "Hauth Hmeta Hreservation") as "H".
+  { eapply delete_reserved_kobj; done. }
+  iModIntro.
+  iDestruct (own_op with "H") as "[Hauth Hreservation]".
+  iFrame.
 Qed.
 
 Lemma update_meta_kobj_vs {γ state used_uid k uid meta} prev_obj obj:
