src/proof/kubernetes_model/inv.v
@@ -5,13 +5,12 @@ From New.proof.k8s_io.apimachinery.pkg.apis.meta Require Export v1.
 From New.proof Require Import prelude empty_ffi.
 From New.proof.kubernetes_types Require Export prelude.
 From New.proof.big_op Require Export big_sepL big_sepM.
-From New.proof.algebra Require Export kview cview tombstone reserved_keys.
+From New.proof.algebra Require Export kview cview terminating_cview.
 
 Class kubernetesModelG Σ := {
   #[global] kubernetes_model_kviewG :: kviewG Σ;
   #[global] kubernetes_model_cviewG :: cviewG Σ;
-  #[global] kubernetes_model_tombstoneG :: tombstoneG Σ;
-  #[global] kubernetes_model_reserved_keysG :: reserved_keysG Σ;
+  #[global] kubernetes_model_terminating_cviewG :: terminating_cviewG Σ;
 }.
 
 Section spec.
@@ -23,8 +22,7 @@ Local Set Default Proof Using "All".
 Record KubernetesGname := mk_γk {
   γ_state : gname;
   γ_children : gname;
-  γ_tombstone : gname;
-  γ_reserved_keys : gname;
+  γ_terminating_children : gname;
 }.
 
 Definition own_kview_auth γ state used_uid : iProp Σ :=
@@ -45,23 +43,20 @@ Definition own_children_auth γ state used_reference : iProp Σ :=
 Definition own_children_frag γ key uid dq keys : iProp Σ :=
   cview.own_frag γ.(γ_children) key uid dq keys.
 
-Definition own_tombstone_auth γ tombed_uid : iProp Σ :=
-  tombstone.own_auth γ.(γ_tombstone) tombed_uid.
+Definition own_terminating_children_auth γ state used_reference : iProp Σ :=
+  terminating_cview.own_auth γ.(γ_terminating_children) state used_reference.
 
-Definition own_tombstone_frag γ tombed_uid : iProp Σ :=
-  tombstone.own_frag γ.(γ_tombstone) tombed_uid.
+Definition own_terminating_children_frag γ key uid dq keys : iProp Σ :=
+  terminating_cview.own_frag γ.(γ_terminating_children) key uid dq keys.
 
-Definition own_reserved_auth γ reserved_key_set : iProp Σ :=
-  reserved_keys.own_auth γ.(γ_reserved_keys) reserved_key_set.
-
-Definition own_reserved_frag γ key : iProp Σ :=
-  reserved_keys.own_frag γ.(γ_reserved_keys) key.
+Definition own_reserved_frag γ key status : iProp Σ :=
+  kview.own_reservation_frag γ.(γ_state) key status.
 
 Definition kubernetes_inv γ l : iProp Σ :=
   ∃ (phys_state_l: loc) (phys_used_uid_l: loc) (phys_used_rv_l: loc)
     (phys_state: gmap KKey.t interface.t) (phys_used_uid : gmap types.UID.t unit) (phys_used_rv : gmap go_string unit)
-    (abs_state: gmap KKey.t KObjectV.t) (used_uid: gset types.UID.t) (tombed_uid: gset types.UID.t)
-    (used_reference: gset (KKey.t * types.UID.t)) (reserved_keys: gset KKey.t),
+    (abs_state: gmap KKey.t KObjectV.t) (used_uid: gset types.UID.t)
+    (used_reference: gset (KKey.t * types.UID.t)),
     "Hstate_m_addr" ∷ l.[(apimodel.State.t), "m"] ↦ phys_state_l ∗
     "Hstate_used_uid_addr" ∷ l.[(apimodel.State.t), "usedUID"] ↦ phys_used_uid_l ∗
     "Hstate_used_rv_addr" ∷ l.[(apimodel.State.t), "usedRV"] ↦ phys_used_rv_l ∗
@@ -70,17 +65,14 @@ Definition kubernetes_inv γ l : iProp Σ :=
     "Hown_used_rv" ∷ phys_used_rv_l ↦$ phys_used_rv ∗
     "Hown_abs" ∷ own_kview_auth γ abs_state used_uid ∗
     "Hown_children" ∷ own_children_auth γ abs_state used_reference ∗
-    "Hown_tombstone" ∷ own_tombstone_auth γ tombed_uid ∗
-    "Hown_reserved" ∷ own_reserved_auth γ reserved_keys ∗
+    "Hown_terminating_children" ∷ own_terminating_children_auth γ abs_state used_reference ∗
     "Hphys_abs_rep" ∷ ([∗ map] i; obj ∈ phys_state; abs_state,
       match i with
       | interface.ok i_ok => KObjectV.deepown_i i_ok obj 1
       | interface.nil => False%I
       end) ∗
     "%Hused_uid_eq_dom_phys_used_uid" ∷ ⌜ used_uid = dom phys_used_uid ⌝ ∗ 
-    "%Hused_uid_eq_set_map_used_reference" ∷ ⌜ used_uid = (set_map (λ v, snd v) used_reference) ⌝ ∗
-    "%Htombed_uid_eq_used_uid_sub" ∷ ⌜ tombed_uid = used_uid ∖ map_to_set (λ _ obj, (KObjectV.objectmeta obj).(ObjectMetaV.UID')) abs_state ⌝ ∗
-    "%Hreserved_disjoint_abs" ∷ ⌜ reserved_keys ## dom abs_state ⌝.
+    "%Hused_uid_eq_set_map_used_reference" ∷ ⌜ used_uid = (set_map (λ v, snd v) used_reference) ⌝.
 
 Definition is_kubernetes γ l : iProp Σ :=
   ∃ (mu_l: loc),
